fix transformation to machine & some injection lemmas

Machine.v
@@ -135,6 +135,28 @@ Definition is_dcall (d:direction) : option nat :=
   | _ => None
   end.
 
+Definition val_injectb (p: prog) (vsrc vtgt: val) : bool :=
+  match vsrc, vtgt with
+  | FP l, N n => match pc_inj p (l, 0) with
+                | Some n' => Nat.eqb n n'
+                | None => false
+                end
+  | N n, N n' => Nat.eqb n n'
+  | UV, _ => true
+  | _, _ => false
+  end.
+
+Definition val_inject (p: prog) (vsrc vtgt: val) : Prop :=
+  match vsrc, vtgt with
+  | FP l, N n => match pc_inj p (l, 0) with
+                | Some n' => (n = n')%nat
+                | None => False
+                end
+  | N n, N n' => (n = n')
+  | UV, _ => True
+  | _, _ => False
+  end.
+
 Module MachineCommon (M: TMap).
 
 Notation "'_' '!->' v" := (M.init v)
@@ -145,6 +167,13 @@ Notation "m '!' x" := (M.t_apply m x)
     (at level 20, left associativity).
 
 Definition reg := M.t val.
+Definition reg_init := M.init UV.
+
+Definition no_fp (r: reg) : Prop :=
+  forall x, match (to_fp (r ! x)) with
+       | Some _ => False
+       | None => True
+       end.
 
 Fixpoint eval (st : reg) (e: exp) : val :=
   match e with
@@ -184,19 +213,56 @@ End MachineCommon.
 
 (* transformation *)
 
+Fixpoint machine_exp (p: prog) (e: exp) : option exp :=
+  match e with
+  | ANum _ | AId _ => Some e
+  | FPtr l => match pc_inj p (l, 0) with
+             | Some l' => Some (ANum l')
+             | None => None
+             end
+  | ABin o e1 e2 => match machine_exp p e1, machine_exp p e2 with
+                   | Some e1', Some e2' => Some (ABin o e1' e2')
+                   | _, _ => None
+                   end
+  | ACTIf e1 e2 e3 => match machine_exp p e1, machine_exp p e2, machine_exp p e3 with
+                     | Some e1', Some e2', Some e3' => Some (ACTIf e1' e2' e3')
+                     | _, _, _ => None
+                     end
+  end.
+
 Definition machine_inst (p: prog) (i: inst) : option inst :=
   match i with
   | <{{branch e to l}}> =>
-      match pc_inj p (l, 0) with
-      | Some l' => Some <{{ branch e to l' }}>
-      | _ => None
-      end
+    match machine_exp p e, pc_inj p (l, 0) with
+    | Some e', Some l' => Some <{{ branch e' to l' }}>
+    | _, _ => None
+    end
   | <{{jump l}}> =>
-      match pc_inj p (l, 0) with
-      | Some l' => Some <{{ jump l' }}>
-      | _ => None
-      end
-  | _ => Some i
+    match pc_inj p (l, 0) with
+    | Some l' => Some <{{ jump l' }}>
+    | _ => None
+    end
+  | ICall e =>
+    match machine_exp p e with
+    | Some e' => Some (ICall e')
+    | _ => None
+    end
+  | IAsgn x e =>
+    match machine_exp p e with
+    | Some e' => Some (IAsgn x e')
+    | _ => None
+    end
+  | ILoad x e =>
+    match machine_exp p e with
+    | Some e' => Some (ILoad x e')
+    | _ => None
+    end
+  | IStore e1 e2 =>
+    match machine_exp p e1, machine_exp p e2 with
+    | Some e1', Some e2' => Some (IStore e1' e2')
+    | _, _ => None
+    end
+  | ISkip | IRet | ICTarget => Some i
   end.
 
 Definition transpose {X : Type} (l : list (option X)) : option (list X) :=
@@ -217,3 +283,45 @@ Definition machine_prog (p: prog) : option prog :=
   let op := map (machine_blk p) p in
   transpose op.
 
+Module SimCommon (M: TMap).
+
+Module MiniC := MiniCETCommon(M).
+Import MiniC.
+
+Module MachineC := MachineCommon(M).
+Import MachineC.
+
+Definition regs := MiniC.reg.
+Definition regt := MachineC.reg.
+
+Definition reg_inject (p: prog) (r1: regs) (r2: regt) : Prop :=
+  forall x, val_inject p (r1 ! x) (r2 ! x).
+
+Lemma eval_binop_inject p o v1 v1' v2 v2'
+    (INJ1: val_inject p v1 v1')
+    (INJ2: val_inject p v2 v2') :
+  val_inject p (eval_binop o v1 v2) (eval_binop o v1' v2').
+Proof.
+  red in INJ1, INJ2. des_ifs. destruct o; ss.
+Admitted.
+
+Lemma eval_inject p r1 r2 e1 e2
+  (INJ: reg_inject p r1 r2)
+  (TRANS: machine_exp p e1 = Some e2) :
+  val_inject p (MiniC.eval r1 e1) (MachineC.eval r2 e2).
+Proof.
+  ginduction e1; ss; ii; clarify.
+  - des_ifs. ss.
+    hexploit IHe1_1; eauto. intros INJ1. hexploit IHe1_2; eauto. intros INJ2.
+    eapply (eval_binop_inject p o); eauto.
+  - des_ifs_safe. hexploit IHe1_1; eauto. i. ss.
+    destruct (MiniC.eval r1 e1_1); ss; auto. des_ifs_safe. ss. clarify.
+    des_ifs.
+    + hexploit IHe1_2; eauto.
+    + hexploit IHe1_3; eauto.
+  - des_ifs. ss. clarify.
+Qed.
+
+(* common simulation *)
+
+End SimCommon.
